ucongr 0.2

uexp/src/uexp/ucongr_lemmas.lean
@@ -4,44 +4,62 @@ import .u_semiring
 section
 variables {s: Schema} {t₁ t₂ t₃: Tuple s} {a b c d e: usr} 
 private meta def simp_solve :=
-    `[intros, simp]
+    `[intros h, rewrite ← h, simp]
 
-lemma usr_eq_symm: a = b → b = a := 
+lemma ueq_symm: a = b → b = a := 
 begin
     intros, rewrite a_1, 
 end
 
 lemma ueq_trans_1 : 
-(t₁ ≃ t₂) * ((t₂ ≃ t₃) * c) * d = (t₁ ≃ t₂) * ((t₂ ≃ t₃) * c) * (d * (t₁ ≃ t₃))  := by simp_solve
+(t₁ ≃ t₂) * ((t₂ ≃ t₃) * c) * (d * (t₁ ≃ t₃)) = e → (t₁ ≃ t₂) * ((t₂ ≃ t₃) * c) * d = e := by simp_solve
 
 lemma ueq_trans_1' : 
-(t₁ ≃ t₂) * (t₂ ≃ t₃) * d = (t₁ ≃ t₂) * (t₂ ≃ t₃) * (d * (t₁ ≃ t₃))  := by simp_solve
+(t₁ ≃ t₂) * (t₂ ≃ t₃) * (d * (t₁ ≃ t₃)) = e → (t₁ ≃ t₂) * (t₂ ≃ t₃) * d = e := by simp_solve
 
 lemma ueq_trans_2_g : 
-(t₁ ≃ t₂) * ((t₁ ≃ t₃) * c) * d = (t₁ ≃ t₂) * ((t₁ ≃ t₃) * c) * (d * (t₂ ≃ t₃))  := by simp_solve
+(t₁ ≃ t₂) * ((t₁ ≃ t₃) * c) * (d * (t₂ ≃ t₃)) = e → (t₁ ≃ t₂) * ((t₁ ≃ t₃) * c) * d = e := by simp_solve
 
 lemma ueq_trans_2_g' : 
-(t₁ ≃ t₂) * (t₁ ≃ t₃) * d = (t₁ ≃ t₂) * (t₁ ≃ t₃) * (d * (t₂ ≃ t₃))  := by simp_solve
+(t₁ ≃ t₂) * (t₁ ≃ t₃) * (d * (t₂ ≃ t₃)) = e → (t₁ ≃ t₂) * (t₁ ≃ t₃) * d = e := by simp_solve
 
 lemma ueq_trans_2_l :
-(t₁ ≃ t₂) * ((t₁ ≃ t₃) * c) * d = (t₁ ≃ t₂) * ((t₁ ≃ t₃) * c) * (d * (t₃  ≃ t₂))  := by simp_solve
+(t₁ ≃ t₂) * ((t₁ ≃ t₃) * c) * (d * (t₃  ≃ t₂)) = e → (t₁ ≃ t₂) * ((t₁ ≃ t₃) * c) * d = e := by simp_solve
 
 lemma ueq_trans_2_l' :
-(t₁ ≃ t₂) * (t₁ ≃ t₃) * d = (t₁ ≃ t₂) * (t₁ ≃ t₃) * (d * (t₃  ≃ t₂))  := by simp_solve
+(t₁ ≃ t₂) * (t₁ ≃ t₃) * (d * (t₃  ≃ t₂)) = e → (t₁ ≃ t₂) * (t₁ ≃ t₃) * d = e := by simp_solve
 
 lemma ueq_trans_3_g :  
-(t₁ ≃ t₂) * ((t₃ ≃ t₂) * c) * d = (t₁ ≃ t₂) * ((t₃ ≃ t₂) * c) * (d * (t₁ ≃ t₃))  := by simp_solve
+(t₁ ≃ t₂) * ((t₃ ≃ t₂) * c) * (d * (t₁ ≃ t₃)) = e → (t₁ ≃ t₂) * ((t₃ ≃ t₂) * c) * d = e := by simp_solve
 
 lemma ueq_trans_3_g' :  
-(t₁ ≃ t₂) * (t₃ ≃ t₂) * d = (t₁ ≃ t₂) * (t₃ ≃ t₂) * (d * (t₁ ≃ t₃))  := by simp_solve
+(t₁ ≃ t₂) * (t₃ ≃ t₂) * (d * (t₁ ≃ t₃)) = e → (t₁ ≃ t₂) * (t₃ ≃ t₂) * d = e := by simp_solve
 
 lemma ueq_trans_3_l :
-(t₁ ≃ t₂) * ((t₃ ≃ t₂) * c) * d = (t₁ ≃ t₂) * ((t₃ ≃ t₂) * c) * (d * (t₃  ≃ t₁))  := by simp_solve
+(t₁ ≃ t₂) * ((t₃ ≃ t₂) * c) * (d * (t₃ ≃ t₁)) = e → (t₁ ≃ t₂) * ((t₃ ≃ t₂) * c) * d = e := by simp_solve
 
 lemma ueq_trans_3_l' :
-(t₁ ≃ t₂) * (t₃ ≃ t₂) * d = (t₁ ≃ t₂) * (t₃ ≃ t₂) * (d * (t₃  ≃ t₁))  := by simp_solve
+(t₁ ≃ t₂) * (t₃ ≃ t₂) * (d * (t₃  ≃ t₁)) = e → (t₁ ≃ t₂) * (t₃ ≃ t₂) * d = e := by simp_solve
+
+lemma ueq_trans_4 :
+(t₁ ≃ t₂) * ((t₃ ≃ t₁) * c) * (d * (t₃ ≃ t₂)) = e → (t₁ ≃ t₂) * ((t₃ ≃ t₁) * c) * d = e := by simp_solve
+
+lemma ueq_trans_4' :
+(t₁ ≃ t₂) * (t₃ ≃ t₁) * (d * (t₃ ≃ t₂)) = e → (t₁ ≃ t₂) * (t₃ ≃ t₁) * d = e := by simp_solve
 
 lemma prod_symm_assoc :
 a * (b * c) = b * (a * c) := by ac_refl 
+
+lemma time_one' :
+1 * a = a := by simp
+
+-- change the goal to the form  a x 1 = b x 1
+lemma add_unit (a b: usr):
+    a * 1 = b * 1 → a = b :=
+begin
+    simp,
+    intros, 
+    assumption,
+end
 
 end -- end section
